
\chapter{Week1}

\section{Wednesday}\index{Wednesday_lecture}
\subsection{Introduction to Imaginary System}
\begin{definition}[Complex Number]
A complex number $z$ is a pair of real numbers:
\[
z = (x,y),
\]
where $x$ is the \emph{real} part and $y$ is the \emph{imaginary part} of $z$, denoted as
\[
\begin{array}{ll}
\mbox{Re}z = x
&
\mbox{Im}z = y
\end{array}
\]
\end{definition}
\begin{remark}
Note that the complex multiplication does not correspond to any standard vector operation. However, $(\mathbb{C},+)$ and $(\mathbb{C}\setminus\{0\},\cdot)$ forms a field:
\begin{align*}
(z_1+z_2)+z_3&=z_1+(z_2+z_3)\\
z_1+z_2&=z_2+z_1\\
z+0&=0+z=z\\
z+(-z)&=(-z)+z=0
\end{align*}
There is no other Eucliean space that can form a field.
\end{remark}
\begin{proposition}
$zz'=0$ if and only if $z=0$ or $z'=0$.
\end{proposition}
\begin{proof}
Rewrite the product as a linear system
\[
\begin{pmatrix}
x&-y\\y&x
\end{pmatrix}\begin{pmatrix}
x'\\y'
\end{pmatrix}=\begin{pmatrix}
0\\0
\end{pmatrix}
\]
and discuss the determinant of the coefficient matrix.
\end{proof}
\paragraph{Solving quadratic equation with one unknown}We can apply the imaginary number to solve the quadratic equations. For example, to solve $z^2-2z+2=0$, the first method is to substitute $z$ with $x+iy$; the second method is to simplify it into standard form to solve it.
\begin{definition} 
If $z\ne0$, then $z^{-1}$ is the complex number satisfying $z\cdot z^{-1}=1$.
\end{definition}
Suppose $z=(x,y)$ and $z^{-1}=(u,v)$. After simplification, we derive
\[
\left\{
\begin{aligned}
xu - yv &=1\\
xv + yu &=0
\end{aligned}
\right.\implies
\left\{
\begin{aligned}
u&=\frac{x}{x^2+y^2}\\
v&=\frac{-y}{x^2+y^2}
\end{aligned}
\right.
\]
\begin{definition}[Division]
The division between complex numbers is defined as:
\[
\begin{array}{ll}
\frac{z_1}{z_2}=z_1\cdot z_2^{-1},
&
\mbox{when }z_2\ne0
\end{array}
\]
\end{definition}
\begin{example}
\[
\frac{3-4i}{1+i} = (3-4i)\left(\frac{1}{2} - \frac{1}{2}i\right)
=-\frac{1}{2} - \frac{7}{2}i
\]
\[
\frac{10}{(1+i)(2+i)(3+i)}=\frac{10}{(1+3i)(3+i)}=\frac{10}{10i}=\frac{1}{i}=-i
\]
\end{example}
\begin{definition}[Complex Conjugate]
The complex number $x-iy$ is called the \emph{complex conjugate} of $z = x+iy$, which is denoted by $\bar z$.
\end{definition}
The following properties hold for complex conjugate:
\[
\begin{array}{lll}
\overline{z_1\pm z_2} = \bar z_1\pm\bar z_2,
&
\overline{z_1z_2} = \bar z_1\bar z_2.
&
\overline{\frac{z_1}{z_2}}=\frac{\bar z_1}{\bar z_2}
\end{array}
\]
\[
\begin{array}{ll}
\mbox{Re}z=\frac{z+\bar z}{2},
&
\mbox{Im}z = \frac{z - \bar z}{2i}
\end{array}
\]
\subsection{Algebraic and geometric properties}
\begin{definition}[Algebraic Region]
\begin{enumerate}
\item
The complex plane: the $z$-plane, i.e., $\mathbb{C}$
\item
Vector in $\mathbb{R}^2$: $(x,y) = x+iy=z\in\mathbb{C}$
\item
Modulus of $z$:
\[
\begin{array}{ll}
|z|=\sqrt{x^2+y^2}
&
\mbox{distance to the origin}
\end{array}
\]
\end{enumerate}
\end{definition}
Note that
\[
\begin{array}{ll}
|z|=0\Longleftrightarrow z=0,
&
|z_1 - z_2| = 0\Longleftrightarrow
z_1=z_2
\end{array}
\]
\begin{definition}[Circle in plane]
A circle with center $z_0$ and radius $R$ is defined as follows in $\mathbb{C}$:
\[
\{z\in\mathbb{C}\mid |z-z_0|=R\}
\]
\end{definition}
\begin{proposition}
Complex roots of polynomials with real coefficients appear in conjugate pairs.
\end{proposition}
\begin{proof}
Given $P(z_0)=0$, we derive
\[
P(z_0)=\overline{P(z_0)}=0.
\]
\end{proof}
Note that a polynomial with real coefficients of degree 3 must have at least one real root.

\paragraph{Conjugate Product}
Note that the conjugate product leads to the square of modulus:
\[
z\cdot\bar z =  |z|^2
\Longleftrightarrow
(x+iy)(x-iy) = x^2 + y^2
\]
Such a property can be used to simplify quotient of two complex numbers:
\[
\frac{z_1}{z_2}=\frac{z_1\bar z_2}{|z_2|^2}=\frac{x_1x_2 + y_1y_2 + (y_1x_2 - x_1y_2)i}{x_2^2+y_2^2}
\]
\begin{example}
\[
\frac{-1+3i}{2-i}=\frac{(-1+3i)(2+i)}{(2-i)(2+i)}=\frac{-5+5i}{5}=-1+i
\]
\[
|z_1+z_2|^2 + |z_1-z_2|^2 = 2(|z_1|^2+|z_2|^2)
\]
\end{example}
We can use conjugate to show the \emph{triangle inequality}:
\begin{proposition}[Triangle Inequality]
$|z_1+z_2|\le|z_1|+ |z_2|$.
\end{proposition}
\begin{proof}
\begin{align*}
|z_1+z_2|^2&=(z_1+z_2)\overline{(z_1+z_2)}\\
&=|z_1|^2+|z_2|^2+z_1\bar z_2 + \overline{z_1\bar z_2}\\
&=|z_1|^2+|z_2|^2+2\mbox{Re}(z_1\bar z_2)\\
&\le |z_1|^2+|z_2|^2+2|z_1\bar z_2|\\
&=|z_1|^2+|z_2|^2+2|z_1z_2|=(|z_1|+|z_2|)^2.
\end{align*}
\end{proof}
\begin{corollary}
\begin{enumerate}
\item
$||z_1| - |z_2||\le |z_1\pm z_2|$.
\item
If $|z|\le 1$, then $|z^2+z+1|\le 3$
\end{enumerate}
\end{corollary}
\begin{proof}
\begin{enumerate}
\item
Note that 
\[
|z_1| = |z_1\pm z_2\mp z_2|\le |z_1\pm z_2|+|z_2|\implies
|z_1|-|z_2|\le |z_1\pm z_2|
\]
Similarly, $|z_2| - |z_1|\le |z_1\pm z_2|$.
\item
\[
|z^2+z+1|\le |z^2|+|z+1|\le |z|^2 + |z|  + 1\le1+1+1=3.
\]
\end{enumerate}
\end{proof}
\begin{proposition}[Cauchy-Schwarz inequality]
If $z_1,\dots,z_n$ and $w_1,\dots,w_n$ are complex numbers, then
\[
\left[
\sum_{k=1}^nz_kw_k
\right]^2
\le
\left[
\sum_{k=1}^n|z_k|^2
\right]
\left[
\sum_{k=1}^n|w_k|^2
\right]
\]
\end{proposition}
\subsection{Polar and exponential forms}
\begin{definition}[Polar Form]
The polar form of a nonzero complex number $z$ is:
\[
z = r(\cos\theta + i\sin\theta)
\]
where $(r,\theta)$ is the polar coordinates of $(x,y)$.
\[
(r,\theta)\implies (x,y):\left\{
\begin{aligned}
x&=r\cos\theta\\
y&=r\sin\theta
\end{aligned}
\right.
\]
\[
(x,y)\implies (r,\theta):\left\{
\begin{aligned}
r&=\sqrt{x^2+y^2}\\
\tan\theta&=\frac{y}{x}
\end{aligned}
\right.
\]
Note that $\theta$ is said to be the \emph{argument} of $z$, i.e., $\theta=\arg z$. The augument is not unique, i.e.,
\[
z = r(\cos\theta + i\sin\theta) 
 r(\cos(\theta+2\pi) + i\sin(\theta + 2\pi))
\]
\end{definition}
If given an argument of $z$, then we form the set of arguments of $z$:
\[
\{\theta+2n\pi\mid n\in\mathbb{Z}\}
\]
\begin{definition}[Principal Value]
The principal value of $\arg z$, denoted by $\mbox{Arg} z$, is the unique value of $\arg z$ such that $-\pi<\arg z\le\pi$
\end{definition}
\begin{example}
\begin{enumerate}
\item
$\mbox{Arg}z=\pi$ implies $z = r(\cos\pi + i\sin\pi) = -r<0$, which is a negative real number.
\item
$\mbox{Arg}z=0$ implies $z=r(\cos0+i\sin0)=r>0$m which is a positive real number.
\item
$\mbox{Arg}z=-\frac{\pi}{2}$ implies $z=r(\cos(-\frac{\pi}{2})+i\sin(-\frac{\pi}{2}))=-ri$
\item
$\mbox{Arg}z = \frac{\pi}{2}$ implies $z = ri$
\item
Particularly, $\pm i = \cos(\pm \frac{\pi}{2}) + i\sin(\pm\frac{\pi}{2})$
\end{enumerate}
\end{example}

\paragraph{Product in polar form}
Given $z_i = r_i(\cos\theta_i+i\sin\theta_i)$ for $i=1,2$, we can compute its product:
\begin{align*}
z_1z_2 &=r_1r_2(\cos\theta_1\cos\theta_2-\sin\theta_1\sin\theta_2 + i(\sin\theta_1\cos\theta_2+\cos\theta_1\sin\theta_2))\\
&=r_1r_2(\cos(\theta_1+\theta_2) + i\sin(\theta_1+\theta_2))
\end{align*}
Thus, $\mbox{arg}(z_1z_2) = \mbox{arg}z_1+\mbox{arg}z_2$.
\begin{remark}
Note that $\mbox{Arg}(z_1z_2)\ne\mbox{Arg}z_1 +\mbox{Arg}z_2$. ($\mbox{Arg}(z_1z_2)$ should be restricted to be within the interval $(-\pi,\pi]$)
\end{remark}

\paragraph{Inverse in Polar form}
Given $z=r(\cos\theta+i\sin\theta)$, we aim to find the inverse such that $zz^{-1}=1$. Hence, $z^{-1}=\frac{1}{r}(\cos(-\theta)+i\sin(-\theta))$.

If we obtain the inverse, we can compute the division $\frac{z_1}{z_2}$:
\[
\frac{z_1}{z_2} =r_1(\cos\theta_1+i\sin\theta_1)\frac{1}{r_2}(\cos(-\theta_2)+i\sin(-\theta_2))
=
\frac{r_1}{r_2}(\cos(\theta_1-\theta_2) + i\sin(\theta_1-\theta_2))
\]
Thus, $\mbox{arg}\frac{z_1}{z_2} =\mbox{arg}z_1 - \mbox{arg}z_2$.

\paragraph{Euler Identity}
The Euler Identity is given by:
\[
e^{ix}  = \cos x+i\sin x
\]
The proof requires Taylor's expansion.

\paragraph{Exponential Form}
The exponential form of $z$ in polar form is given by:
\[
z = re^{i\theta}
\]
Then it is convenient to define produt, inverse, and division:
\begin{align*}
(r_1e^{i\theta_1})\cdot(r_2e^{i\theta_2})&=
r_1r_2e^{i(\theta_1+\theta_2)}\\
\frac{1}{re^{i\theta}}&=\frac{1}{r}e^{i(-\theta)}\\
\frac{r_1e^{i\theta_1}}{r_2e^{i\theta_2}}&=\frac{r_1}{r_2}e^{i(\theta_1-\theta_2)}
\end{align*}

\paragraph{Nonuniqueness} $z=re^{i\theta} = re^{i(\theta+2n\pi)}$


\paragraph{Equality} Two complex numbers are equal means that:
\[
r_1e^{i\theta_1}=r_2e^{i\theta_2}
\Longleftrightarrow
\left\{
\begin{aligned}
r_1&=r_2\\
\theta_1&=\theta_2+2k\pi,k\in\mathbb{Z}
\end{aligned}
\right.
\]

\paragraph{Circle} The circle centered at the origin with radius $R$ can be describled as:
\[
\begin{array}{ll}
|z| = R\Longleftrightarrow z = Re^{i\theta},
&
0\le\theta<2\pi
\end{array}
\]
The circle centered at $z_0$ with radius $R$ can be describled as:
\[
\begin{array}{ll}
|z-z_0| = R\Longleftrightarrow z = z_0+Re^{i\theta},
&
0\le\theta<2\pi
\end{array}
\]

\paragraph{Neighborhoold} The $\epsilon$-neighborhood of the point $z_0$ is given by:
\[
\begin{array}{l}
|z-z_0| < \epsilon
\end{array}
\]
If delete the center, it is given by:
\[
\begin{array}{l}
0<|z-z_0| < \epsilon
\end{array}
\]



\section{Powers and Roots}
\paragraph{Powers}
The powers of $z=re^{i\theta}$ is given by:
\begin{align*}
z^n&=r^ne^{in\theta}\\
z^{-n} = r^{-n}e^{i(-n)\theta}
\end{align*}
Thus we derive the \emph{De Moiver's Formula}:
\[
(\cos\theta+i\sin\theta)^n=(e^{i\theta})^n
=\cos n\theta+i\sin n\theta.
\]
It is useful for computing powers tha contains complex number. For example,
\[
(1+i)^n = (\sqrt{2}e^{i\frac{\pi}{4}})^n
=2^{n/2}e^{\frac{in\pi}{4}}
\]
\begin{proposition}
\[
\sin(n\theta) = \sum_{k=0}^{\lfloor{n/2}\rfloor}\binom{n}{2k+1}(-1)^k\cos^{n-2k-1}\theta\sin^{2k+1}\theta,
\]
where $\lfloor{x}\rfloor$ denotes the largest integer that not exceeds $x$.
\end{proposition}
\paragraph{Solving high order equations}The powers of complex can also be used to solve high order equations.
\begin{example}
To sovle the equation $z^n=1$, we express $z = re^{i\theta}$. It follows that
\[
(re^{i\theta})^n = 1e^{i0}\implies
\left\{
\begin{aligned}
r^n&=1\\
n\theta&=2k\pi
\end{aligned}\right.
\implies
\left\{
\begin{aligned}
r&=1\\
\theta&=\frac{2k\pi}{n}
\end{aligned}\right.
\]
Thus, the distinct $n$-th roots( of unity) are given by:
\[
\exp(i\frac{2k\pi}{n}) = \cos\frac{2k\pi}{n} + i\sin\frac{2k\pi}{n},\qquad
k=0,1,2,\dots,n-1.
\]
If we denote $w_n=\exp(i\frac{2\pi}{n})$, we derive the roots:
\[
1,w_n,w_n^2,\dots,w_n^{n-1}.
\]
\end{example}
\paragraph{Roots of high order equations}
Suppose $z_0=r_0e^{i\theta_0}$, we aim to sovle $z^n = z_0$:
\[
r^ne^{in\theta} = r_0e^{i\theta_0}\implies
\left\{
\begin{aligned}
r&=r_0^{1/n}\\
\theta&=\frac{\theta_0+2k\pi}{n}
\end{aligned}
\right.
\]
Thus the distinct $n$th roots are given by:
\[
r_0^{1/n}\exp(i\frac{\theta_0+2k\pi}{n}),\qquad
k=0,1,2,\dots,n-1.
\]
If $c$ is any particular $n$-th roots of $z_0$, then
\[
(cw)^n=z_0\implies
c^nw^n=z_0\implies w_n=1.
\]
Hence, the distinct $n$-th roots of $z_0$ are
\[
c,cw_n,cw_n^2,\dots,cw_n^{n-1}
\]
\begin{remark}
\begin{itemize}
\item
There are $n$ of the $n$-th roots of a complex number, all the roots are equally spaced about a circle that is centered at origin with radius $|z_0|^{1/n}$.
\item
Let $z_0^{1/n}$ denote the set of all $n$-th roots of $z_0$. If $\theta_0=\mbox{Arg}z_0$, then
\[
c_0=r_0^{1/n}\exp(i\frac{\theta_0}{n})
\]
is called the principal $n$-th root of $z_0$.
\item
The distinct $n$-th roots of $z_0$ are:
\[
c_0,c_0w_n,c_ow_n^2,\dots,c_0w_n^{n-1},
\]
or equivalently,
\[
z_0^{1/n} = r_0^{1/n}\exp(i\frac{\theta_0+2k\pi}{n})
\]
\end{itemize}

\end{remark}

\begin{example}
For $z_0= -8i$, we write $z_0=8e^{i(-\pi/2)}$. It follows that
\[
z_0^{1/3} = =2\exp(i\frac{-\pi/2 + 2k\pi}{3}) = 2\exp(-\frac{\pi}{6}i),2\exp(\frac{\pi}{2}i),2\exp(\frac{7\pi}{6}i)
\]

\end{example}
