\chapter{Introduction to Linear Programming}

\section{Preliminaries}
\paragraph{Standard Form}
We usually consider the standard linear programming (LP) model:
\begin{equation}\label{Eq:1:1}
\begin{array}{ll}
\max&\sum_{j=1}^nc_jx_j\\
\text{s.t.}&\sum_{j=1}^na_{ij}x_j\le b_i,\quad i=1,\dots,m\\
&x_j\ge 0, j=1,\dots,n
\end{array}
\end{equation}

Or more generally, the constraints with equalities:
\begin{equation*}
\begin{array}{ll}
\min&\sum_{j=1}^nc_jx_j\\
\text{s.t.}&\sum_{j=1}^na_{ij}x_j\le b_i,\quad i\in I\\
&\sum_{j=1}^na_{ij}x_j= b_i,\quad i\in E\\
&x_j\ge 0, j=1,\dots,n
\end{array}
\end{equation*}

It's often convenient to write the LP~(\ref{Eq:1:1}) into the compact matrix form:
\begin{equation}
\begin{array}{ll}
\max&\bm c\trans\bm x\\
\text{s.t.}&\bm{Ax}\le\bm b\\
&\bm x\ge\bm0
\end{array}
\end{equation}
where $\bm c\in\mathbb{R}^n,\bm A\in\mathbb{R}^{m\times n},\bm b\in\mathbb{R}^m$.

We also write $\bm A$ as the column form:
\[
\bm A=\begin{pmatrix}
\bm a_1,&\cdots&\bm a_n
\end{pmatrix}
\]
where $\bm a_i$ is the $i$-th column of $\bm A$. We also express the submatrix of $\bm A$, i.e., $\bm A_I\subset A$ as:
\[
\bm A_I:=[a_i\mid i\in I],
\]
where $I$ is a subset of $\{1,2,\dots,n\}$.

\paragraph{Dictionaries of an LP}
We can introduce slack variables to transform (\ref{Eq:1:1}) into LP with equalities:
\[
x_{n+i}:=b_i - \sum_{j=1}^na_{ij}x_j,\quad i=1,\dots,m
\]
Let $z=\sum_{j=1}^nc_jx_j$ be the objective function, and therefore we obtain a \emph{dictionary} for the LP~(\ref{Eq:1:1}):
\begin{equation}
\left.
\begin{aligned}
x_{n+i}&=b_i - \sum_{j=1}^na_{ij}x_j,\quad i=1,\dots,m\\
z&=\sum_{j=1}^nc_jx_j
\end{aligned}
\right\}\qquad \text{Dictionary}
\end{equation}

Assume that $b_i\ge0$ for $i=1,\dots,m$. Therefore we obtain a \emph{feasible solution} associated with the dictionary, say \emph{dictionary solution}:
\[
\begin{array}{ll}
x_j=0,\ \text{for $j=1,\dots,n$}
&
x_{n+i}=b_i \ \text{for $i=1,\dots,m$}
\end{array}
\]

It's clear how to improve the current dictionary solution:
\begin{itemize}
\item
If $c_j\le0,\forall j$, then we cannot possibly improve the dictionary solution
\item
If $c_j>0$ for some $1\le j\le n$, we increase the value for $x_j$ from $0$ into maximal value, while fixing $x_j=0$ for $1\le k(\ne j)\le n$. Keep implementing until $c_j\le0,\forall j$.
\end{itemize}

\begin{example}
\begin{subequations}
Consider the optimization problem
\begin{equation}
\begin{array}{ll}
\max&5x_1+4x_2+3x_3\\
\text{s.t.}&2x_1+3x_2+x_3\le 5\\
&4x_1+x_2+2x_3\le 11\\
&3x_1+4x_2+2x_3\le 8\\
&x_1\ge0,\ x_2\ge0, \ x_3\ge0
\end{array}
\end{equation}
We can find its dictionary:
\begin{equation}
\begin{aligned}
x_4&=5\bm{-2}x_1-3x_2-x_3\\
x_5&=11-4x_1-x_2-2x_3\\
x_6&=8-3x_1-4x_2-2x_3\\
z&=0\bm{+5}x_1+4x_2+3x_3
\end{aligned}
\end{equation}
Since $c_1>0$, increasing value for $x_1$ suffices to consider the dictionary below instead:
\begin{equation}
\begin{aligned}
x_1&=\frac{5}{2}-\frac{3}{2}x_2-\frac{1}{2}x_3-\frac{1}{2}x_4\\
x_5&=11-4x_1-x_2-2x_3\\
x_6&=8-3x_1-4x_2-2x_3\\
z&=0+5x_1+4x_2+3x_3
\end{aligned}
\Longleftrightarrow
\begin{aligned}
x_1&=\frac{5}{2}-\frac{3}{2}x_2-\frac{1}{2}x_3-\frac{1}{2}x_4\\
x_5&=1+5x_2+0x_3+2x_4\\
x_6&=\frac{1}{2}+\frac{1}{2}x_2-\frac{1}{2}x_3+\frac{3}{2}x_4\\
z&=\frac{25}{2}-\frac{7}{2}x_2+\frac{1}{2}x_3-\frac{5}{2}x_4
\end{aligned}
\end{equation}
Also, since $c_3>0$, increasing value for $x_3$ suffices to consider the dictionary below instead:
\begin{equation}
\begin{aligned}
x_1&=\frac{5}{2}-\frac{3}{2}x_2-\frac{1}{2}x_3-\frac{1}{2}x_4\\
x_5&=1+5x_2+0x_3+2x_4\\
x_3&=1+x_2+3x_4-2x_6\\
z&=\frac{25}{2}-\frac{7}{2}x_2+\frac{1}{2}x_3-\frac{5}{2}x_4
\end{aligned}
\Longleftrightarrow
\begin{aligned}
x_3&=1+x_2+3x_4-2x_6\\
x_1&=2-x_2-2x_4+x_6\\
x_5&=1+5x_2+2x_4+2x_6\\
z&=13-3x_2-x_4-x_6
\end{aligned}
\end{equation}

\end{subequations}
\end{example}

\section{Simplex Method}

\paragraph{Notations}
The general dictionary for the problem~(\ref{Eq:1:1}) can be expressed as:
\begin{equation}\label{Eq:1:5}
\begin{aligned}
x_i&=\bar b_i -\sum_{j\in N}\bar{a}_{ij}x_j,\quad i\in B\\
z&=\zeta - \sum_{j\in N}\bar c_jx_j
\end{aligned}
\end{equation}
where
\begin{enumerate}
\item
the set $B$ is called a \emph{basis}, with $|B|=m$
\item
the set $N$ is called a \emph{non-basis}, with $|N|=n-m$. Moreover, $B\cupdot N = \{1,\dots,n\}$.
\item
the basis $B$ is said to be \emph{primal feasible} if $\bar{\bm b}\ge0$, since in this case we can choose a primal feasible solution by setting non-basis variables to be zero and basis variables $x_i$ to be $\bar{b}_i$.
\item
the non-basis $N$ is said to be \emph{dual feasible} if $\bar{\bm c}\le 0$, since in this case we can choose a dual feasible solution by setting non-basis variables to be $\bar{c}_i$ and other variables to be $0$.
\end{enumerate}
One can verify that in (\ref{Eq:1:5}), 
\begin{align*}
\bar{\bm b}&=\bm A_B^{-1}\bm b\\
\bar{\bm c}_N\trans&=\bm c_N\trans - \bm c_B\trans\bm A_B^{-1}\bm A_N\\
\bar{\bm A}_N&=\bm A_B^{-1}\bm A_N\\
\zeta&=\bm c_B\trans\bm A_B^{-1}\bm b
\end{align*}
One can verify that $(\bm x_B,\bm x_N)=(\bm A_B^{-1}\bm b,\bm0)$ is a \emph{basic solution}.

\paragraph{Simplex Method Algorithm}
The assumption for the working of simplex method is that we are given a primal feasible basic solution, i.e., $\bar{b}\ge0$. The framework for obtaining an improved solution is summarized in (\ref{alg:SM}).


\begin{algorithm}[htb] 
\caption{Framework for the one step of the Simplex Method} 
\label{alg:SM} 
\begin{algorithmic}[1] %show number in each rows
\REQUIRE ~~\\ %算法的输入参数：Input
Primal feasible basic solution;
\ENSURE ~~\\ %算法的输出：Output
Improved feasible basic solution;
\STATE Entering Basis Variable
\begin{itemize}
\item
Search for $j\in N$ such that $\bar{c}_j>0$
\item
If none exists then the current basic solution is optimal; otherwise choose one of such $j$.
\end{itemize}
\STATE Leaving Basis Variable
\begin{itemize}
\item
Search for $i\in B$ such that $\bar{a}_{ij}>0$
\item
If none exists then the problem is unbounded; otherwise choose
\[
i\in\arg\min\left\{\frac{\bar{b}_i}{\bar{a}_{ij}}: \bar{a}_{ij}>0,\ i\in B
\right\}
\]
\end{itemize}
\label{code:fram:trainbase}
\STATE Basis Update:  $B\leftarrow B\cup\{j\}\setminus\{i\}$, and then form the corresponding basic solution.
\end{algorithmic}
\end{algorithm}
\begin{remark}
The \emph{one-step} of the simplex method is also called a \emph{pivot step}, i.e., choose one pivot variable entering the basis and one leaving the basis.

The objective value for a successful pivot is improved by $\frac{\bar{c}_j\bar{b}_i}{\bar{a}_{ij}}$. However, the simplex method may not necessarily increase the objective value at each pivot, e.g., the case $\bar{b}_i=0$ coul happen. In this case, the basic solution is said to be \emph{degenerate}.

Since there are no more than $\binom{n}{m}$ (finite) possible bases, the simplex method will stop on two cases: (a) declaring the problem is unbounded; (b) finding a basic optimal solution.
\end{remark}
\paragraph{Pivot Rules}
The \emph{simplex method} specializes into a \emph{simplex algorithm} if one specifies a \emph{pivot rule} to determine which one variable to enter the basis and which one to leave, when there is a choice to make. Note that there exists some pivot rules that will make the problem face into cycling circumstance (see the example below), but here we list some examples of pivot rules that will be shown to definitely avoid cycling circumstance:
\begin{itemize}
\item
Dantzig’s pivot rule: \emph{choose the largest positive coefficient to enter the basis.}
\item
The maximum improvement rule: \emph{try all the combinations and pick the pivot pair with the largest improvement}.
\item
Bland's rule: \emph{Among the candidates always pick the one with the smallest index}.
\end{itemize}

\begin{example}
This example shows that some pivot rules may let the problem face into cycling circumstance, i.e., the algorithm solves the problem in a loop and fails to go out:
\begin{align*}
\bm{x_5}&=-0.5x_1+5.5x_2+2.5x_3-9x_4\\
x_6&=-0.5x_1+1.5x_2+0.5x_3-x_4\\
x_7&=1-x_1\\
z&=\bm{10x_1}-57x_2-9x_3-24x_4
\end{align*}
Choosing $x_1$ to enter the basis and $x_5$ to leave gives:
\begin{align*}
x_1&=-2x_5+11x_2+5x_3-18x_4\\
\bm{x_6}&=x_5-4x_2-2x_3+8x_4\\
x_7&=1+2x_5-11x_2-5x_3+18x_4\\
z&=-20x_5+\bm{53x_2}+41x_3-204x_4
\end{align*}
Choosing $x_2$ to enter the basis and $x_6$ to leave gives:
\begin{align*}
\bm{x_1}&=0.75x_5-2.75x_6-0.5x_3+4x_4\\
x_2&=0.25x_5-0.25x_6-0.5x_3+2x_4\\
x_7&=1-0.75x_5-13.25x_6+0.5x_3-4x_4\\
z&=-6.75x_5-13.25x_6+\bm{14.5x_3}-98x_4
\end{align*}
Choosing $x_3$ to enter the basis and $x_1$ to leave gives:
\begin{align*}
x_3&=1.5x_5-5.5x_5-2x_1+8x_4\\
\bm{x_2}&=-0.5x_5+2.5x_5+x_1-2x_4\\
x_7&=1-x_1\\
z&=15x_5-93x_5-29x_1+\bm{18x_4}
\end{align*}
Choosing $x_4$ to enter the basis and $x_2$ to leave gives:
\begin{align*}
\bm{x_3}&=-0.5x_5+4.5x_5+2x_1-4x_2\\
x_4&=-0.25x_5+1.25x_5+0.5x_1-0.5x_2\\
x_7&=1-x_1\\
z&=\bm{10.5x_5}-70.5x_5-20x_1-9x_2
\end{align*}
Choosing $x_5$ to enter the basis and $x_3$ to leave gives:
\begin{align*}
x_5&=9x_6+4x_1-8x_2-2x_3\\
\bm{x_4}&=-x_6-0.5x_1+1.5x_2+0.5x_3\\
x_7&=1-x_1\\
z&=\bm{24x_6}+22x_1-93x_2-21x_3
\end{align*}
Choosing $x_6$ to enter the basis and $x_4$ to leave gives the \emph{same dictionary as we started}:
\begin{align*}
\bm{x_5}&=-0.5x_1+5.5x_2+2.5x_3-9x_4\\
x_6&=-0.5x_1+1.5x_2+0.5x_3-x_4\\
x_7&=1-x_1\\
z&=\bm{10x_1}-57x_2-9x_3-24x_4
\end{align*}
\end{example}

\begin{theorem}
Bland's pivot rule would aviod cycling.
\end{theorem}
\begin{proof}
We show this claim by contradiction. If Bland's pivot rule produces cycling, let's study one cycle. For a sequence of dictionaries that form a cycle, let's delete all the variables that neither leave nor enter the basis, then it will remain a cycle.

In all these dictionaries, all $\bar{b}_i$ will be zero, since otherwise the objective value will be strictly increased.

Let's study the tablau of dictionaries. It's a matrix that stores all the coefficients of a dictionary:
\[
\begin{array}{cc|c}
\hline
  \bm I_B & \bm A_B^{-1}\bm A_N&\bar{\bm b} \\ \hline
  \bm 0\trans&\bar{\bm c}_N\trans&\bm c_B\trans\bm A_B^{-1}\bm b \\ \hline
\end{array}
\]
Two vectors are of special interest. The last row of the tablau in left part can be written as
\[
\bar{\bm c}\trans=\bm c - \bm c_B\trans\bm A_B^{-1}\bm A
\]
For the chosen $j\in N$, the direction
\[
d_i^{(j)} = \left\{
\begin{aligned}
-\bar{a}_{ij},&\quad i\in B\\
0&,\quad i\ne j\\
1&,\quad i=j
\end{aligned}
\right.
\]
It's clear that $\bar{\bm c}\trans \bm d^{(j)}=\bar{c}_j$.

Suppose that $\ell$ is the largest index of all variables that are involved in the cycle. Let $(B,N)$ be the pivot where $\ell$ was about to enter the basis, $\bm v=\bar{\bm c}$ be the last row for that tableau at that point; let $(B',N')$ be the pivot where $\ell$ was about to leave the basis, and $k$ was to enter the basis at that point, $\bm d^{(k)}$ be the corresponding direction vector, $\bm u$ the last row of that tableau.

It's clear that 
\begin{itemize}
\item
$\bm v$ is everywhere non-positive except for one position $v_\ell>0$
\item
$\bm d^{(k)}$ is everywhere non-negative except for one position $d_\ell^{(k)}<0$
\end{itemize}
Moreover, $\bm v-\bm u\in\mathcal{R}(\bm A\trans)$ and $\bm d^{(k)}\in\mathcal{N}(\bm A)$, which implies
\[
0 = (\bm v-\bm u)\trans \bm d^{(k)} = \bm v\trans\bm d^{(k)} - \bm u_k<0,
\]
which is a contradiction.
\end{proof}






















